benchmark/benchmark_compute.v
@@ -1,0 +1,23 @@
+From Coq Require Import NArith.
+From mathcomp Require Import all_ssreflect.
+From stablesort Require Import stablesort.
+From benchmark Require Import benchmark.
+
+Elpi sort_benchmark
+  "compute" "compute" (map (N.mul 100) (N_iota 1 40))
+  "CBN.sort1"    (eager_bench CBN.sort1)
+  "CBN.sort2"    (eager_bench CBN.sort2)
+  "CBN.sort3"    (eager_bench CBN.sort3)
+  "CBN.sortN"    (eager_bench CBN.sortN)
+  "CBNAcc.sort1" (eager_bench CBNAcc.sort1)
+  "CBNAcc.sort2" (eager_bench CBNAcc.sort2)
+  "CBNAcc.sort3" (eager_bench CBNAcc.sort3)
+  "CBNAcc.sortN" (eager_bench CBNAcc.sortN)
+  "CBV.sort1"    (eager_bench CBV.sort1)
+  "CBV.sort2"    (eager_bench CBV.sort2)
+  "CBV.sort3"    (eager_bench CBV.sort3)
+  "CBV.sortN"    (eager_bench CBV.sortN)
+  "CBVAcc.sort1" (eager_bench CBVAcc.sort1)
+  "CBVAcc.sort2" (eager_bench CBVAcc.sort2)
+  "CBVAcc.sort3" (eager_bench CBVAcc.sort3)
+  "CBVAcc.sortN" (eager_bench CBVAcc.sortN).
