benchmark/extraction.v
@@ -15,10 +15,10 @@ Extract Inlined Constant eqb => "(Prelude.==)".
 
 Extract Inductive list => "([])" ["([])" "(:)"].
 
-Extraction "benchmark/MergesortCoqCbn.hs" CBN.sort.
-Extraction "benchmark/MergesortCoqCbnOpt.hs" CBNOpt.sort.
-Extraction "benchmark/MergesortCoqCbv.hs" CBV.sort.
-Extraction "benchmark/MergesortCoqCbvOpt.hs" CBVOpt.sort.
+Extraction "benchmark/haskell/MergesortCoqCbn.hs"    CBN.
+Extraction "benchmark/haskell/MergesortCoqCbnAcc.hs" CBNAcc.
+Extraction "benchmark/haskell/MergesortCoqCbv.hs"    CBV.
+Extraction "benchmark/haskell/MergesortCoqCbvAcc.hs" CBVAcc.
 
 (******************************************************************************)
 
@@ -34,5 +34,4 @@ Extract Inductive list => "list" ["[]" "(::)"].
 Extract Inlined Constant catrev => "List.rev_append".
 Extract Inlined Constant rev => "List.rev".
 
-Extraction "benchmark/mergesort_coq.ml"
-           CBN.sort CBNOpt.sort CBV.sort CBVOpt.sort.
+Extraction "benchmark/ocaml/mergesort_coq.ml" CBN CBNAcc CBV CBVAcc.
